chore: make EncodeAscii ghost

AwsCryptographicMaterialProviders/dafny/AwsCryptographicMaterialProviders/test/CMCs/LocalCMC.dfy
@@ -47,11 +47,19 @@ module  {:options "/functionSyntax:4"} TestLocalCMC {
     )
   }
 
+const abc : UTF8.ValidUTF8Bytes := 
+  var s := [0x61, 0x62, 0x63];
+  assert s == UTF8.EncodeAscii("abc");
+  s
+
+const cde : UTF8.ValidUTF8Bytes := 
+  var s := [0x63, 0x64, 0x65];
+  assert s == UTF8.EncodeAscii("cde");
+  s
+
   method {:test} LocalCMCBasics() {
     var st := new LocalCMC(100);
 
-    var abc := UTF8.EncodeAscii("abc");
-    var cde := UTF8.EncodeAscii("cde");
     var res := st.GetCacheEntryWithTime(MakeGet(abc), 10000);
     expect res.Failure?;
     expect res.error.EntryDoesNotExist?;
